Nlp/Core/Data.lean
@@ -1,5 +1,6 @@
 import Nlp.Core.Data.Span
 import Nlp.Core.Data.ChartLayout
+import Nlp.Core.Data.Dependency
 import Nlp.Core.Data.FloatArrayExt
 import Nlp.Core.Data.FloatChart
 import Nlp.Core.Data.Interner
